Refactor proof of KVS search to reduce compilation load

theories/case_studies/multiuser_kvs/kvs_spec_search.v
@@ -14,6 +14,582 @@ Section KVS_search.
     {swlayout : switcherLayout}
   .
 
+  Definition kvs_search_found_resources `{KVS : kvsLayout}
+    (pc_b pc_e pc_a cgp_b cgp_e : Addr)
+    (rkey ridx ridx_empty rscratch : RegName)
+    (pkvs : kvs_physical_map) (idx : nat) (fkey : full_key_t) (w : Word) : iProp Σ :=
+    let instrs := kvs_search_instrs rkey ridx ridx_empty rscratch in
+    (PC ↦ᵣ WCap RX Global pc_b pc_e (pc_a ^+ length instrs)%a ∗
+     cgp ↦ᵣ WCap RW Global cgp_b cgp_e
+       (cgp_b ^+ (ASM_SIZEOF_KVS_ENTRY * idx))%a ∗
+     rkey ↦ᵣ WInt fkey ∗ ridx ↦ᵣ WInt idx ∗ ridx_empty ↦ᵣ - ∗ rscratch ↦ᵣ - ∗
+     (cgp_b ^+ (ASM_SIZEOF_KVS_ENTRY * idx))%a ↦ₐ WInt ASM_SOME ∗
+     (cgp_b ^+ (ASM_SIZEOF_KVS_ENTRY * idx + 1))%a ↦ₐ WInt fkey ∗
+     (cgp_b ^+ (ASM_SIZEOF_KVS_ENTRY * idx + 2))%a ↦ₐ w ∗
+     is_physical_kvs_open cgp_b pkvs idx ∗
+     ⌜withinBounds cgp_b cgp_e
+        (cgp_b ^+ (ASM_SIZEOF_KVS_ENTRY * idx + 2))%a = true⌝ ∗
+     codefrag pc_a instrs)%I.
+
+  Definition kvs_search_missing_resources `{KVS : kvsLayout}
+    (pc_b pc_e pc_a cgp_b cgp_e : Addr)
+    (rkey ridx ridx_empty rscratch : RegName)
+    (pkvs : kvs_physical_map) (fkey : full_key_t) : iProp Σ :=
+    let instrs := kvs_search_instrs rkey ridx ridx_empty rscratch in
+    ((∃ idx_empty_slot : nat,
+       PC ↦ᵣ WCap RX Global pc_b pc_e (pc_a ^+ length instrs)%a ∗
+       cgp ↦ᵣ WCap RW Global cgp_b cgp_e cgp_b ∗
+       rkey ↦ᵣ WInt fkey ∗ ridx ↦ᵣ WInt (-1)%Z ∗
+       ridx_empty ↦ᵣ WInt idx_empty_slot ∗ rscratch ↦ᵣ - ∗
+       is_physical_kvs_open cgp_b pkvs idx_empty_slot ∗
+       (cgp_b ^+ (ASM_SIZEOF_KVS_ENTRY * idx_empty_slot))%a ↦ₐ WInt ASM_NONE ∗
+       (cgp_b ^+ (ASM_SIZEOF_KVS_ENTRY * idx_empty_slot + 1))%a ↦ₐ - ∗
+       (cgp_b ^+ (ASM_SIZEOF_KVS_ENTRY * idx_empty_slot + 2))%a ↦ₐ - ∗
+       ⌜withinBounds cgp_b cgp_e
+          (cgp_b ^+ (ASM_SIZEOF_KVS_ENTRY * idx_empty_slot + 2))%a = true⌝ ∗
+       ⌜0 <= idx_empty_slot⌝ ∗
+       ⌜pkvs !! idx_empty_slot = Some None⌝ ∗ codefrag pc_a instrs) ∨
+     (PC ↦ᵣ WCap RX Global pc_b pc_e (pc_a ^+ length instrs)%a ∗
+      cgp ↦ᵣ WCap RW Global cgp_b cgp_e cgp_b ∗
+      rkey ↦ᵣ WInt fkey ∗ ridx ↦ᵣ WInt (-1)%Z ∗
+      ridx_empty ↦ᵣ WInt (-1)%Z ∗ rscratch ↦ᵣ - ∗
+      is_physical_kvs cgp_b pkvs ∗ codefrag pc_a instrs))%I.
+
+  Lemma kvs_physical_map_open_any
+    (a : Addr) (pkvs : kvs_physical_map) (idx : nat) :
+    0 <= idx < SIZE_MAP ->
+    is_physical_kvs a pkvs -∗
+    ∃ opt_kw,
+      ⌜pkvs !! idx = Some opt_kw⌝ ∗
+      is_physical_kvs_open a pkvs idx ∗
+      physical_kvs_entry a idx opt_kw.
+  Proof.
+    iIntros (Hidx) "[%Hwf HKVS]".
+    pose proof (wf_kvs_is_Some pkvs idx Hwf Hidx) as [opt_kw Hlookup].
+    iExists opt_kw. iSplit; first done.
+    rewrite -{1}(insert_id pkvs idx opt_kw); last done.
+    iDestruct (big_sepM_insert_delete with "HKVS") as "[Hentry HKVS]".
+    iFrame. iPureIntro; done.
+  Qed.
+
+  Lemma kvs_search_empty_iteration_spec `{KVS : kvsLayout}
+    (pc_b pc_e pc_a cgp_b cgp_e : Addr)
+    (rkey ridx ridx_empty rscratch : RegName) (n fkey : Z)
+    (wempty wscratch w1 w2 : Word) :
+    let instrs := kvs_search_instrs rkey ridx ridx_empty rscratch in
+    SubBounds pc_b pc_e pc_a (pc_a ^+ length instrs)%a ->
+    ((cgp_b + (ASM_SIZEOF_KVS_ENTRY * SIZE_MAP)%Z)%a = Some cgp_e)%a ->
+    (0 <= n < SIZE_MAP)%Z ->
+    rscratch ≠ cnull ->
+    ridx ≠ cnull ->
+    ridx_empty ≠ cnull ->
+    rkey ≠ cnull ->
+
+    (PC ↦ᵣ WCap RX Global pc_b pc_e (pc_a ^+ 2)%a ∗
+     cgp ↦ᵣ WCap RW Global cgp_b cgp_e
+       (cgp_b ^+ (ASM_SIZEOF_KVS_ENTRY * n))%a ∗
+     rkey ↦ᵣ WInt fkey ∗
+     ridx ↦ᵣ WInt n ∗
+     ridx_empty ↦ᵣ wempty ∗
+     rscratch ↦ᵣ wscratch ∗
+     (cgp_b ^+ (ASM_SIZEOF_KVS_ENTRY * n))%a ↦ₐ WInt ASM_NONE ∗
+     (cgp_b ^+ (ASM_SIZEOF_KVS_ENTRY * n + 1))%a ↦ₐ w1 ∗
+     (cgp_b ^+ (ASM_SIZEOF_KVS_ENTRY * n + 2))%a ↦ₐ w2 ∗
+     codefrag pc_a instrs ∗
+
+     ▷ (PC ↦ᵣ WCap RX Global pc_b pc_e (pc_a ^+ 2)%a ∗
+        cgp ↦ᵣ WCap RW Global cgp_b cgp_e
+          (cgp_b ^+ (ASM_SIZEOF_KVS_ENTRY * (n + 1)))%a ∗
+        rkey ↦ᵣ WInt fkey ∗
+        ridx ↦ᵣ WInt (n + 1) ∗
+        ridx_empty ↦ᵣ WInt n ∗
+        rscratch ↦ᵣ WInt 0 ∗
+        (cgp_b ^+ (ASM_SIZEOF_KVS_ENTRY * n))%a ↦ₐ WInt ASM_NONE ∗
+        (cgp_b ^+ (ASM_SIZEOF_KVS_ENTRY * n + 1))%a ↦ₐ w1 ∗
+        (cgp_b ^+ (ASM_SIZEOF_KVS_ENTRY * n + 2))%a ↦ₐ w2 ∗
+        codefrag pc_a instrs -∗
+        WP Seq (Instr Executable) {{ v, ⌜v = HaltedV⌝ → na_own cerise_nais ⊤ }})
+     ⊢ WP Seq (Instr Executable) {{ v, ⌜v = HaltedV⌝ → na_own cerise_nais ⊤ }})%I.
+  Proof.
+    intros instrs HsubBounds Hcgp_bound Hn Hrscratch Hridx Hridx_empty Hkey.
+    iIntros "(HPC & Hcgp & Hrkey & Hridx & Hempty & Hscratch & Hn0 & Hn1 & Hn2 & Hcode & Hpost)".
+    codefrag_facts "Hcode"; rename H into Hpc_contiguous; clear H0.
+    (* sub rscratch SIZE_MAP ridx; *)
+    iInstr "Hcode".
+    assert (WInt (SIZE_MAP - n) ≠ WInt 0) by (injection; intro; lia).
+    (* jnz (".loop_body")%asm rscratch; *)
+    iInstr "Hcode".
+    (* load rscratch cgp; *)
+    iInstr "Hcode". { split; [done | solve_addr]. }
+    (* jnz (".some_index")%asm rscratch; *)
+    iInstr "Hcode".
+    (* mov ridx_empty ridx; *)
+    iInstr "Hcode".
+    (* lea cgp ASM_SIZEOF_KVS_ENTRY; *)
+    iInstr "Hcode".
+    { transitivity (Some (cgp_b ^+ (ASM_SIZEOF_KVS_ENTRY * (n + 1)))%a); solve_addr. }
+    (* add ridx ridx 1; *)
+    iInstr "Hcode".
+    (* jmp (".loop_start")%asm; *)
+    iInstr "Hcode". { transitivity (Some (pc_a ^+ 2)%a); solve_addr. }
+    iApply "Hpost". iFrame.
+  Qed.
+
+  Lemma kvs_search_found_iteration_spec `{KVS : kvsLayout}
+    (pc_b pc_e pc_a cgp_b cgp_e : Addr)
+    (rkey ridx ridx_empty rscratch : RegName)
+    (n fkey kidx : Z) (widx wempty wscratch : Word) :
+    let instrs := kvs_search_instrs rkey ridx ridx_empty rscratch in
+    SubBounds pc_b pc_e pc_a (pc_a ^+ length instrs)%a ->
+    ((cgp_b + (ASM_SIZEOF_KVS_ENTRY * SIZE_MAP)%Z)%a = Some cgp_e)%a ->
+    (0 <= n < SIZE_MAP)%Z ->
+    rscratch ≠ cnull ->
+    ridx ≠ cnull ->
+    ridx_empty ≠ cnull ->
+    rkey ≠ cnull ->
+
+    (PC ↦ᵣ WCap RX Global pc_b pc_e (pc_a ^+ 2)%a ∗
+     cgp ↦ᵣ WCap RW Global cgp_b cgp_e
+       (cgp_b ^+ (ASM_SIZEOF_KVS_ENTRY * n))%a ∗
+     rkey ↦ᵣ WInt fkey ∗
+     ridx ↦ᵣ WInt n ∗
+     ridx_empty ↦ᵣ wempty ∗
+     rscratch ↦ᵣ wscratch ∗
+     (cgp_b ^+ (ASM_SIZEOF_KVS_ENTRY * n))%a ↦ₐ WInt ASM_SOME ∗
+     (cgp_b ^+ (ASM_SIZEOF_KVS_ENTRY * n + 1))%a ↦ₐ WInt kidx ∗
+     (cgp_b ^+ (ASM_SIZEOF_KVS_ENTRY * n + 2))%a ↦ₐ widx ∗
+     codefrag pc_a instrs ∗
+
+     ▷ (((⌜fkey = kidx⌝ ∗
+           PC ↦ᵣ WCap RX Global pc_b pc_e (pc_a ^+ length instrs)%a ∗
+           cgp ↦ᵣ WCap RW Global cgp_b cgp_e
+             (cgp_b ^+ (ASM_SIZEOF_KVS_ENTRY * n))%a ∗
+           rkey ↦ᵣ WInt fkey ∗
+           ridx ↦ᵣ WInt n ∗
+           ridx_empty ↦ᵣ wempty ∗
+           rscratch ↦ᵣ WInt 0 ∗
+           (cgp_b ^+ (ASM_SIZEOF_KVS_ENTRY * n))%a ↦ₐ WInt ASM_SOME ∗
+           (cgp_b ^+ (ASM_SIZEOF_KVS_ENTRY * n + 1))%a ↦ₐ WInt kidx ∗
+           (cgp_b ^+ (ASM_SIZEOF_KVS_ENTRY * n + 2))%a ↦ₐ widx ∗
+           codefrag pc_a instrs) ∨
+          (⌜fkey ≠ kidx⌝ ∗
+           PC ↦ᵣ WCap RX Global pc_b pc_e (pc_a ^+ 2)%a ∗
+           cgp ↦ᵣ WCap RW Global cgp_b cgp_e
+             (cgp_b ^+ (ASM_SIZEOF_KVS_ENTRY * (n + 1)))%a ∗
+           rkey ↦ᵣ WInt fkey ∗
+           ridx ↦ᵣ WInt (n + 1) ∗
+           ridx_empty ↦ᵣ wempty ∗
+           rscratch ↦ᵣ WInt (fkey - kidx) ∗
+           (cgp_b ^+ (ASM_SIZEOF_KVS_ENTRY * n))%a ↦ₐ WInt ASM_SOME ∗
+           (cgp_b ^+ (ASM_SIZEOF_KVS_ENTRY * n + 1))%a ↦ₐ WInt kidx ∗
+           (cgp_b ^+ (ASM_SIZEOF_KVS_ENTRY * n + 2))%a ↦ₐ widx ∗
+           codefrag pc_a instrs)) -∗
+        WP Seq (Instr Executable) {{ v, ⌜v = HaltedV⌝ → na_own cerise_nais ⊤ }})
+     ⊢ WP Seq (Instr Executable) {{ v, ⌜v = HaltedV⌝ → na_own cerise_nais ⊤ }})%I.
+  Proof.
+    intros instrs HsubBounds Hcgp_bound Hn Hrscratch Hridx Hridx_empty Hkey.
+    iIntros "(HPC & Hcgp & Hrkey & Hridx & Hempty & Hscratch & Hn0 & Hn1 & Hn2 & Hcode & Hpost)".
+    codefrag_facts "Hcode"; rename H into Hpc_contiguous; clear H0.
+    (* sub rscratch SIZE_MAP ridx; *)
+    iInstr "Hcode".
+    assert (WInt (SIZE_MAP - n) ≠ WInt 0) by (injection; intro; lia).
+    (* jnz (".loop_body")%asm rscratch; *)
+    iInstr "Hcode".
+    (* load rscratch cgp; *)
+    iInstr "Hcode".
+    { split; [done | solve_addr]. }
+    (* jnz (".some_index")%asm rscratch; *)
+    iInstr "Hcode".
+    (* lea cgp 1; *)
+    iInstr "Hcode".
+    { transitivity (Some (cgp_b ^+ (ASM_SIZEOF_KVS_ENTRY * n + 1))%a); [solve_addr | done]. }
+    (* load rscratch cgp; *)
+    iInstr "Hcode".
+    { split; [done | solve_addr]. }
+    (* sub rscratch rkey rscratch; *)
+    iInstr "Hcode".
+    destruct (decide (fkey = kidx)) as [-> | Hneq].
+    - replace (kidx - kidx)%Z with 0%Z by lia.
+      (* jnz (".not_same_key")%asm rscratch; *)
+      iInstr "Hcode".
+      (* lea cgp (-1)%Z; *)
+      iInstr "Hcode"; first (transitivity (Some (cgp_b ^+ (ASM_SIZEOF_KVS_ENTRY * n))%a); solve_addr).
+      (* jmp (".loop_end_found")%asm; *)
+      iInstr "Hcode".
+      iApply "Hpost". iLeft. iFrame. done.
+    - assert (WInt (fkey - kidx)%Z ≠ WInt 0) by (injection; intro; simplify_eq; apply Hneq; lia).
+      (* jnz (".not_same_key")%asm rscratch; *)
+      iInstr "Hcode".
+      (* lea cgp 2; *)
+      iInstr "Hcode"; first (transitivity (Some (cgp_b ^+ (ASM_SIZEOF_KVS_ENTRY * (n + 1)))%a); [solve_addr | done]).
+      (* add ridx ridx 1; *)
+      iInstr "Hcode".
+      (* jmp (".loop_start")%asm; *)
+      iInstr "Hcode"; first (transitivity (Some (pc_a ^+ 2)%a); solve_addr).
+      iApply "Hpost". iRight. iFrame. done.
+  Qed.
+
+  Definition kvs_search_outcome_resources `{KVS : kvsLayout}
+    (pc_b pc_e pc_a cgp_b cgp_e : Addr)
+    (rkey ridx ridx_empty rscratch : RegName)
+    (pkvs : kvs_physical_map) (fkey : full_key_t) : iProp Σ :=
+    ((∃ (idx : nat) (w : Word),
+       ⌜pkvs !! idx = Some (Some (fkey, w))⌝ ∗
+       kvs_search_found_resources pc_b pc_e pc_a cgp_b cgp_e
+         rkey ridx ridx_empty rscratch pkvs idx fkey w) ∨
+     (⌜fkey ∉ kvs_keys pkvs⌝ ∗
+      kvs_search_missing_resources pc_b pc_e pc_a cgp_b cgp_e
+        rkey ridx ridx_empty rscratch pkvs fkey))%I.
+
+  Lemma kvs_search_full_block_spec `{KVS : kvsLayout}
+    (pc_b pc_e pc_a cgp_b cgp_e : Addr)
+    (rkey ridx ridx_empty rscratch : RegName) (fkey : full_key_t)
+    (wempty wscratch : Word) :
+    let instrs := kvs_search_instrs rkey ridx ridx_empty rscratch in
+    SubBounds pc_b pc_e pc_a (pc_a ^+ length instrs)%a ->
+    withinBounds cgp_b cgp_e cgp_b = true ->
+    ((cgp_b + (ASM_SIZEOF_KVS_ENTRY * SIZE_MAP)%Z)%a = Some cgp_e)%a ->
+    rscratch ≠ cnull ->
+    ridx ≠ cnull ->
+    ridx_empty ≠ cnull ->
+    rkey ≠ cnull ->
+
+    (PC ↦ᵣ WCap RX Global pc_b pc_e (pc_a ^+ 2)%a ∗
+     cgp ↦ᵣ WCap RW Global cgp_b cgp_e cgp_e ∗
+     rkey ↦ᵣ WInt fkey ∗
+     ridx ↦ᵣ WInt SIZE_MAP ∗
+     ridx_empty ↦ᵣ wempty ∗
+     rscratch ↦ᵣ wscratch ∗
+     codefrag pc_a instrs ∗
+
+     ▷ (PC ↦ᵣ WCap RX Global pc_b pc_e (pc_a ^+ length instrs)%a ∗
+        cgp ↦ᵣ WCap RW Global cgp_b cgp_e cgp_b ∗
+        rkey ↦ᵣ WInt fkey ∗
+        ridx ↦ᵣ WInt (-1)%Z ∗
+        ridx_empty ↦ᵣ wempty ∗
+        rscratch ↦ᵣ WInt 0 ∗
+        codefrag pc_a instrs -∗
+        WP Seq (Instr Executable) {{ v, ⌜v = HaltedV⌝ → na_own cerise_nais ⊤ }})
+     ⊢ WP Seq (Instr Executable) {{ v, ⌜v = HaltedV⌝ → na_own cerise_nais ⊤ }})%I.
+  Proof.
+    intros instrs HsubBounds Hbounds_cgp Hcgp_bound Hrscratch Hridx Hridx_empty Hkey.
+    iIntros "(HPC & Hcgp & Hrkey & Hridx & Hempty & Hscratch & Hcode & Hpost)".
+    codefrag_facts "Hcode"; rename H into Hpc_contiguous; clear H0.
+    (* sub rscratch SIZE_MAP ridx; *)
+    iInstr "Hcode".
+    replace (SIZE_MAP - SIZE_MAP)%Z with 0%Z by lia.
+    (* jnz (".loop_body")%asm rscratch; *)
+    iInstr "Hcode".
+    (* jmp (".loop_end_not_found")%asm; *)
+    iInstr "Hcode".
+    (* lea cgp (-(ASM_SIZEOF_KVS_ENTRY*SIZE_MAP))%Z; *)
+    iInstr "Hcode".
+    { transitivity (Some cgp_b); rewrite /SIZE_MAP in Hcgp_bound |- *; solve_addr. }
+    (* mov ridx (-1)%Z; *)
+    iInstr "Hcode".
+    rewrite (decide_False (Z.of_nat 0)); last done.
+    iApply "Hpost". iFrame.
+  Qed.
+
+  Lemma KVS_search_unified_spec `{KVS : kvsLayout}
+    (pc_b pc_e pc_a cgp_b cgp_e : Addr)
+    (rkey ridx ridx_empty rscratch : RegName)
+    (pkvs : kvs_physical_map) (fkey : full_key_t) :
+    let instrs := kvs_search_instrs rkey ridx ridx_empty rscratch in
+    SubBounds pc_b pc_e pc_a (pc_a ^+ length instrs)%a ->
+    withinBounds cgp_b cgp_e cgp_b = true ->
+    ((cgp_b + (ASM_SIZEOF_KVS_ENTRY * SIZE_MAP)%Z)%a = Some cgp_e)%a ->
+    rscratch ≠ cnull -> ridx ≠ cnull -> ridx_empty ≠ cnull -> rkey ≠ cnull ->
+    (PC ↦ᵣ WCap RX Global pc_b pc_e pc_a ∗
+     cgp ↦ᵣ WCap RW Global cgp_b cgp_e cgp_b ∗
+     rkey ↦ᵣ WInt fkey ∗ ridx ↦ᵣ - ∗ ridx_empty ↦ᵣ - ∗ rscratch ↦ᵣ - ∗
+     is_physical_kvs cgp_b pkvs ∗ codefrag pc_a instrs ∗
+     ▷ (kvs_search_outcome_resources pc_b pc_e pc_a cgp_b cgp_e
+          rkey ridx ridx_empty rscratch pkvs fkey -∗
+        WP Seq (Instr Executable) {{ v, ⌜v = HaltedV⌝ → na_own cerise_nais ⊤ }})
+     ⊢ WP Seq (Instr Executable) {{ v, ⌜v = HaltedV⌝ → na_own cerise_nais ⊤ }})%I.
+  Proof.
+    intros instrs.
+    iIntros (HsubBounds Hbounds_cgp Hcgp_bound Hrscratch Hridx Hridx_empty Hkey)
+      "(HPC & Hcgp & Hrkey & [%wridx Hridx] & [%wridx_empty Hridx_empty] & Hrscratch
+        & HKVS & Hcode & Hpost)".
+    codefrag_facts "Hcode"; rename H into Hpc_contiguous; clear H0.
+    iDestruct (is_physical_kvs_wf with "HKVS") as %Hwf_pkvs.
+
+    (* mov ridx 0%Z; *)
+    iInstr "Hcode".
+    (* mov ridx_empty (-1)%Z; *)
+    iInstr "Hcode".
+    destruct (decide (ridx_empty = cnull)) as [Hnull | Hnonnull]; first done.
+
+    remember 0%Z as n.
+    iAssert (⌜ (0 <= n <= SIZE_MAP)%Z ⌝)%I as "%Hn"; first (iPureIntro ; lia).
+    rewrite{2} (_ : cgp_b = (cgp_b ^+ (ASM_SIZEOF_KVS_ENTRY * n))%a); last by solve_addr.
+    assert (forall i, (0 <= i < Z.to_nat n) -> ∀ (k : Z) (w : Word), pkvs !! i = Some (Some (k,w)) -> k ≠ fkey)
+    as Hfkey_notin_nfirst.
+    { rewrite Heqn; intros i Hi; lia. }
+
+    iAssert (
+       if (decide ((Forall (fun idx => pkvs !! idx ≠ Some None) (seq 0 (Z.to_nat n)))))
+       then (is_physical_kvs cgp_b pkvs ∗
+             ridx_empty ↦ᵣ WInt (-1)
+            )
+       else ( ∃ (idx_empty : nat),
+                ⌜ 0 <= idx_empty < (Z.to_nat n)⌝ ∗
+                is_physical_kvs_open cgp_b pkvs idx_empty ∗
+                (cgp_b ^+ ASM_SIZEOF_KVS_ENTRY * idx_empty)%a ↦ₐ WInt ASM_NONE ∗
+                (cgp_b ^+ (ASM_SIZEOF_KVS_ENTRY * idx_empty + 1))%a ↦ₐ - ∗
+                (cgp_b ^+ (ASM_SIZEOF_KVS_ENTRY * idx_empty + 2))%a ↦ₐ - ∗
+                ridx_empty ↦ᵣ WInt idx_empty ∗
+                ⌜ pkvs !! idx_empty = Some None ⌝
+            )
+      )%I with "[HKVS Hridx_empty]" as "Hloop_inv".
+    {
+      destruct ( decide (Forall (λ idx : nat, pkvs !! idx ≠ Some None) (seq 0 (Z.to_nat n))) ) as [|Hcontra]; iFrame.
+      exfalso; apply Hcontra.
+      rewrite Heqn /=; apply Forall_nil; done.
+    }
+    clear Heqn.
+
+    iLöb as "IH" forall (n Hn Hfkey_notin_nfirst).
+
+    iDestruct "Hrscratch" as "[%wrscratch Hrscratch]".
+    destruct (decide ((SIZE_MAP - n) = 0)%Z) as [Hneq|Hneq].
+    { (* End of the loop. *)
+      assert (n = SIZE_MAP) as -> by lia.
+      replace (cgp_b ^+ (ASM_SIZEOF_KVS_ENTRY * SIZE_MAP))%a with cgp_e by
+        (rewrite /SIZE_MAP in Hcgp_bound |- *; solve_addr).
+      assert (fkey ∉ kvs_keys pkvs) as Hnotin.
+      { intro Hin. apply elem_of_kvs_keys in Hin as (w0 & idx0 & Hlookup).
+        eapply (Hfkey_notin_nfirst idx0); eauto.
+        pose proof (wf_kvs_indom_idx pkvs idx0) as Hidx0.
+        apply Hidx0; [by apply elem_of_dom | done]. }
+      destruct ( decide ( (Forall (λ idx : nat, pkvs !! idx ≠ Some None) (seq 0 (Z.to_nat SIZE_MAP))) )) as [Hnone|Hnone].
+      - iDestruct "Hloop_inv" as "(HKVS & Hridx_empty)".
+        iApply (kvs_search_full_block_spec pc_b pc_e pc_a cgp_b cgp_e
+          rkey ridx ridx_empty rscratch fkey (WInt (-1)) wrscratch
+          HsubBounds Hbounds_cgp Hcgp_bound Hrscratch Hridx Hridx_empty Hkey
+          with "[$HPC $Hcgp $Hrkey $Hridx $Hridx_empty $Hrscratch $Hcode HKVS Hpost]").
+        iNext. iIntros "(HPC & Hcgp & Hrkey & Hridx & Hridx_empty & Hrscratch & Hcode)".
+        iApply "Hpost".
+        rewrite /kvs_search_outcome_resources /kvs_search_missing_resources.
+        iRight. iSplit; first done. iRight. iFrame.
+
+      - iDestruct "Hloop_inv" as
+          "(%idx_empty_found & %Hidx_empty_found & HKVS & Hn0 & Hn1 & Hn2 & Hridx_empty & %Hpkvs_idx_empty)".
+        iApply (kvs_search_full_block_spec pc_b pc_e pc_a cgp_b cgp_e
+          rkey ridx ridx_empty rscratch fkey (WInt idx_empty_found) wrscratch
+          HsubBounds Hbounds_cgp Hcgp_bound Hrscratch Hridx Hridx_empty Hkey
+          with "[$HPC $Hcgp $Hrkey $Hridx $Hridx_empty $Hrscratch $Hcode HKVS Hn0 Hn1 Hn2 Hpost]").
+        iNext. iIntros "(HPC & Hcgp & Hrkey & Hridx & Hridx_empty & Hrscratch & Hcode)".
+        iApply "Hpost".
+        rewrite /kvs_search_outcome_resources /kvs_search_missing_resources.
+        iRight. iSplit; first done. iLeft. iFrame.
+        iPureIntro; split.
+        * solve_addr.
+        * split; [lia | exact Hpkvs_idx_empty].
+    }
+    assert (0 ≤ n < SIZE_MAP)%Z as Hn' by lia.
+
+    destruct ( decide (Forall (λ idx : nat, pkvs !! idx ≠ Some None) (seq 0 (Z.to_nat n))) ) as [Hnone | Hnone].
+    - (* No empty slot have been found yet *)
+      iDestruct "Hloop_inv" as "(HKVS & Hridx_empty)".
+
+      iDestruct (kvs_physical_map_open_any _ _ (Z.to_nat n) with "HKVS")
+        as "(%opt_kwidx & %Hm_kwidx & HKVS & Hfkey)"; first lia.
+      iDestruct (destruct_physical_kvs_entry with "Hfkey") as "(Hn0 & Hn1 & Hn2)"; first solve_addr.
+      replace (cgp_b ^+ ASM_SIZEOF_KVS_ENTRY * Z.to_nat n)%a  with (cgp_b ^+ (ASM_SIZEOF_KVS_ENTRY * n))%a by solve_addr+Hn.
+      replace (cgp_b ^+ (ASM_SIZEOF_KVS_ENTRY * Z.to_nat n + 1))%a with (cgp_b ^+ (ASM_SIZEOF_KVS_ENTRY * n + 1))%a by solve_addr+Hn.
+      replace (cgp_b ^+ (ASM_SIZEOF_KVS_ENTRY * Z.to_nat n + 2))%a with (cgp_b ^+ (ASM_SIZEOF_KVS_ENTRY * n + 2))%a by solve_addr+Hn.
+
+      destruct opt_kwidx as [ [kidx widx] | ].
+      + (* This is not an empty slot. Because we mkow that fkey ∉ s, the key will not match *)
+        iApply (kvs_search_found_iteration_spec pc_b pc_e pc_a cgp_b cgp_e
+          rkey ridx ridx_empty rscratch n fkey kidx widx (WInt (-1)) wrscratch
+          HsubBounds Hcgp_bound Hn' Hrscratch Hridx Hridx_empty Hkey
+          with "[$HPC $Hcgp $Hrkey $Hridx $Hridx_empty $Hrscratch $Hn0 $Hn1 $Hn2 $Hcode HKVS Hpost]").
+        iNext. iIntros "Hresult".
+        iDestruct "Hresult" as "[(%Hsame & HPC & Hcgp & Hrkey & Hridx & Hridx_empty & Hrscratch & Hn0 & Hn1 & Hn2 & Hcode) |
+          (%Hdifferent & HPC & Hcgp & Hrkey & Hridx & Hridx_empty & Hrscratch & Hn0 & Hn1 & Hn2 & Hcode)]".
+        { subst kidx.
+          iApply "Hpost".
+          rewrite /kvs_search_outcome_resources /kvs_search_found_resources.
+          iLeft. iExists (Z.to_nat n), widx. iSplit; first done.
+          assert (Hnat : Z.of_nat (Z.to_nat n) = n) by lia.
+          rewrite Hnat.
+          iFrame. iPureIntro; solve_addr+Hn Hn' Hcgp_bound. }
+
+        iDestruct (kvs_physical_map_close with "[$HKVS] [Hn0 Hn1 Hn2]") as "HKVS";eauto.
+        {
+          iApply destruct_physical_kvs_entry; first solve_addr.
+          replace (cgp_b ^+ (ASM_SIZEOF_KVS_ENTRY * n))%a with (cgp_b ^+ ASM_SIZEOF_KVS_ENTRY * Z.to_nat n)%a by solve_addr+Hn.
+          replace (cgp_b ^+ (ASM_SIZEOF_KVS_ENTRY * n + 1))%a  with (cgp_b ^+ (ASM_SIZEOF_KVS_ENTRY * Z.to_nat n + 1))%a by solve_addr+Hn.
+          replace (cgp_b ^+ (ASM_SIZEOF_KVS_ENTRY * n + 2))%a  with (cgp_b ^+ (ASM_SIZEOF_KVS_ENTRY * Z.to_nat n + 2))%a by solve_addr+Hn.
+          iFrame.
+        }
+        iApply ("IH" with "[] [] [$Hcgp] [$Hrkey] [$Hrscratch]
+         [$Hpost] [$Hridx] [$Hcode] [$HPC] [HKVS Hridx_empty]").
+        * iPureIntro; lia.
+        * iPureIntro.
+          intros idx0 Hidx0_bound k0 w0 Hidx0.
+          destruct (decide (idx0 = Z.to_nat n)%Z) as [-> | Hidx']; eauto.
+          { rewrite Hm_kwidx in Hidx0; simplify_map_eq; done. }
+          { eapply Hfkey_notin_nfirst; eauto; lia. }
+        * case_decide as Hnone'; iFrame.
+          exfalso.
+          apply Hnone'.
+          replace ( (seq 0 (Z.to_nat (n + 1))) ) with ( (seq 0 (Z.to_nat n)) ++ [Z.to_nat n] ).
+          2: {
+            replace [Z.to_nat n] with (seq (Z.to_nat n) 1) by done.
+            rewrite -seq_app.
+            replace (Z.to_nat n + 1) with (Z.to_nat (n + 1)) by lia.
+            done.
+          }
+          apply Forall_app; split; auto.
+          apply Forall_singleton.
+          rewrite Hm_kwidx; done.
+      + (* This is an empty slot. We will update ridx_empty and keep KVS open *)
+        iDestruct "Hn1" as "[%wn1 Hn1]".
+        iDestruct "Hn2" as "[%wn2 Hn2]".
+        iApply (kvs_search_empty_iteration_spec pc_b pc_e pc_a cgp_b cgp_e
+          rkey ridx ridx_empty rscratch n fkey (WInt (-1)) wrscratch wn1 wn2
+          HsubBounds Hcgp_bound Hn' Hrscratch Hridx Hridx_empty Hkey
+          with "[$HPC $Hcgp $Hrkey $Hridx $Hridx_empty $Hrscratch $Hn0 $Hn1 $Hn2 $Hcode HKVS Hpost]").
+        iNext. iIntros "Hresult".
+        iDestruct "Hresult" as "(HPC & Hcgp & Hrkey & Hridx & Hridx_empty & Hrscratch & Hn0 & Hn1 & Hn2 & Hcode)".
+
+        replace n with (Z.of_nat (Z.to_nat n)) in Hridx_empty by lia.
+        replace (cgp_b ^+ (ASM_SIZEOF_KVS_ENTRY * n))%a with (cgp_b ^+ ASM_SIZEOF_KVS_ENTRY * Z.to_nat n)%a by solve_addr+Hn.
+        replace (cgp_b ^+ (ASM_SIZEOF_KVS_ENTRY * n + 1))%a  with (cgp_b ^+ (ASM_SIZEOF_KVS_ENTRY * Z.to_nat n + 1))%a by solve_addr+Hn.
+        replace (cgp_b ^+ (ASM_SIZEOF_KVS_ENTRY * n + 2))%a  with (cgp_b ^+ (ASM_SIZEOF_KVS_ENTRY * Z.to_nat n + 2))%a by solve_addr+Hn.
+        iApply ("IH" with "[] [] [$Hcgp] [$Hrkey] [$Hrscratch]
+         [$Hpost] [$Hridx] [$Hcode] [$HPC] [HKVS Hridx_empty Hn0 Hn1 Hn2]").
+        * iPureIntro; lia.
+        * iPureIntro.
+          intros idx0 Hidx0_bound k0 w0 Hidx0.
+          destruct (decide (idx0 = Z.to_nat n)%Z) as [-> | Hidx']; eauto.
+          { rewrite Hm_kwidx in Hidx0; simplify_map_eq; done. }
+          { eapply Hfkey_notin_nfirst; eauto; lia. }
+        * case_decide as Hnone'.
+          { iFrame. exfalso.
+            replace ( (seq 0 (Z.to_nat (n + 1))) ) with ( (seq 0 (Z.to_nat n)) ++ [Z.to_nat n] ) in Hnone'.
+            2: {
+              replace [Z.to_nat n] with (seq (Z.to_nat n) 1) by done.
+              rewrite -seq_app.
+              replace (Z.to_nat n + 1) with (Z.to_nat (n + 1)) by lia.
+              done.
+            }
+            apply Forall_app in Hnone' as [_ Hnone'].
+            apply (Forall_singleton _ (Z.to_nat n)) in Hnone'; cbn in *.
+            done. }
+          iExists (Z.to_nat n). iSplit; first (iPureIntro; lia).
+          iFrame.
+          replace (Z.of_nat (Z.to_nat n)) with n by lia. iFrame.
+          iPureIntro; exact Hm_kwidx.
+
+    - (* An empty slot have already been found *)
+      iDestruct "Hloop_inv" as
+        "(%idx_empty_found & %Hidx_empty_found & HKVS & Hn0 & Hn1 & Hn2 & Hridx_empty
+          & %Hpkvs_idx_empty)".
+
+      iDestruct (kvs_physical_map_close _ _ _ None with "[$HKVS] [Hn0 Hn1 Hn2]") as "HKVS";eauto.
+      { iApply destruct_physical_kvs_entry; first solve_addr; iFrame. }
+
+
+      iDestruct (kvs_physical_map_open_any _ _ (Z.to_nat n) with "HKVS")
+        as "(%opt_kwidx & %Hm_kwidx & HKVS & Hfkey)"; first lia.
+      iDestruct (destruct_physical_kvs_entry with "Hfkey") as "(Hn0 & Hn1 & Hn2)"; first solve_addr.
+      replace (cgp_b ^+ ASM_SIZEOF_KVS_ENTRY * Z.to_nat n)%a  with (cgp_b ^+ (ASM_SIZEOF_KVS_ENTRY * n))%a by solve_addr+Hn.
+      replace (cgp_b ^+ (ASM_SIZEOF_KVS_ENTRY * Z.to_nat n + 1))%a with (cgp_b ^+ (ASM_SIZEOF_KVS_ENTRY * n + 1))%a by solve_addr+Hn.
+      replace (cgp_b ^+ (ASM_SIZEOF_KVS_ENTRY * Z.to_nat n + 2))%a with (cgp_b ^+ (ASM_SIZEOF_KVS_ENTRY * n + 2))%a by solve_addr+Hn.
+
+      destruct opt_kwidx as [ [kidx widx] | ].
+      + (* This is not an empty slot. Because we mkow that fkey ∉ s, the key will not match *)
+        iApply (kvs_search_found_iteration_spec pc_b pc_e pc_a cgp_b cgp_e
+          rkey ridx ridx_empty rscratch n fkey kidx widx (WInt idx_empty_found) wrscratch
+          HsubBounds Hcgp_bound Hn' Hrscratch Hridx Hridx_empty Hkey
+          with "[$HPC $Hcgp $Hrkey $Hridx $Hridx_empty $Hrscratch $Hn0 $Hn1 $Hn2 $Hcode HKVS Hpost]").
+        iNext. iIntros "Hresult".
+        iDestruct "Hresult" as "[(%Hsame & HPC & Hcgp & Hrkey & Hridx & Hridx_empty & Hrscratch & Hn0 & Hn1 & Hn2 & Hcode) |
+          (%Hdifferent & HPC & Hcgp & Hrkey & Hridx & Hridx_empty & Hrscratch & Hn0 & Hn1 & Hn2 & Hcode)]".
+        { subst kidx.
+          iApply "Hpost".
+          rewrite /kvs_search_outcome_resources /kvs_search_found_resources.
+          iLeft. iExists (Z.to_nat n), widx. iSplit; first done.
+          assert (Hnat : Z.of_nat (Z.to_nat n) = n) by lia.
+          rewrite Hnat.
+          iFrame. iPureIntro; solve_addr+Hn Hn' Hcgp_bound. }
+
+        iDestruct (kvs_physical_map_close with "[$HKVS] [Hn0 Hn1 Hn2]") as "HKVS";eauto.
+        {
+          iApply destruct_physical_kvs_entry; first solve_addr.
+          replace (cgp_b ^+ (ASM_SIZEOF_KVS_ENTRY * n))%a with (cgp_b ^+ ASM_SIZEOF_KVS_ENTRY * Z.to_nat n)%a by solve_addr+Hn.
+          replace (cgp_b ^+ (ASM_SIZEOF_KVS_ENTRY * n + 1))%a  with (cgp_b ^+ (ASM_SIZEOF_KVS_ENTRY * Z.to_nat n + 1))%a by solve_addr+Hn.
+          replace (cgp_b ^+ (ASM_SIZEOF_KVS_ENTRY * n + 2))%a  with (cgp_b ^+ (ASM_SIZEOF_KVS_ENTRY * Z.to_nat n + 2))%a by solve_addr+Hn.
+          iFrame.
+        }
+        iDestruct (kvs_physical_map_open_any _ _ idx_empty_found with "HKVS")
+          as "(%opt_kwidx_empty & %Hm_kwidx_empty & HKVS & Hfkey)"; first lia.
+        rewrite Hpkvs_idx_empty in Hm_kwidx_empty; simplify_eq.
+        iDestruct (destruct_physical_kvs_entry with "Hfkey") as "(Hn0 & Hn1 & Hn2)"; first solve_addr.
+
+        iApply ("IH" with "[] [] [$Hcgp] [$Hrkey] [$Hrscratch]
+         [$Hpost] [$Hridx] [$Hcode] [$HPC] [HKVS Hn0 Hn1 Hn2 Hridx_empty]").
+        * iPureIntro; lia.
+        * iPureIntro.
+          intros idx0 Hidx0_bound k0 w0 Hidx0.
+          clear Hidx_empty_found.
+          destruct (decide (idx0 = Z.to_nat n)%Z) as [-> | Hidx']; eauto.
+          { rewrite Hm_kwidx in Hidx0; simplify_map_eq; done. }
+          { eapply Hfkey_notin_nfirst; eauto; lia. }
+        * case_decide as Hnone'; iFrame; last (iPureIntro; split; auto; lia).
+          exfalso.
+          rewrite Forall_forall in Hnone'.
+          specialize (Hnone' idx_empty_found).
+          apply Hnone'; auto.
+          apply elem_of_seq; lia.
+
+
+      + (* This is an empty slot. We will update ridx_empty and keep KVS open *)
+        iDestruct "Hn1" as "[%wn1 Hn1]".
+        iDestruct "Hn2" as "[%wn2 Hn2]".
+        iApply (kvs_search_empty_iteration_spec pc_b pc_e pc_a cgp_b cgp_e
+          rkey ridx ridx_empty rscratch n fkey (WInt idx_empty_found) wrscratch wn1 wn2
+          HsubBounds Hcgp_bound Hn' Hrscratch Hridx Hridx_empty Hkey
+          with "[$HPC $Hcgp $Hrkey $Hridx $Hridx_empty $Hrscratch $Hn0 $Hn1 $Hn2 $Hcode HKVS Hpost]").
+        iNext. iIntros "Hresult".
+        iDestruct "Hresult" as "(HPC & Hcgp & Hrkey & Hridx & Hridx_empty & Hrscratch & Hn0 & Hn1 & Hn2 & Hcode)".
+        replace n with (Z.of_nat (Z.to_nat n)) in Hridx_empty by lia.
+        replace (cgp_b ^+ (ASM_SIZEOF_KVS_ENTRY * n))%a with (cgp_b ^+ ASM_SIZEOF_KVS_ENTRY * Z.to_nat n)%a by solve_addr+Hn.
+        replace (cgp_b ^+ (ASM_SIZEOF_KVS_ENTRY * n + 1))%a  with (cgp_b ^+ (ASM_SIZEOF_KVS_ENTRY * Z.to_nat n + 1))%a by solve_addr+Hn.
+        replace (cgp_b ^+ (ASM_SIZEOF_KVS_ENTRY * n + 2))%a  with (cgp_b ^+ (ASM_SIZEOF_KVS_ENTRY * Z.to_nat n + 2))%a by solve_addr+Hn.
+        iApply ("IH" with "[] [] [$Hcgp] [$Hrkey] [$Hrscratch]
+         [$Hpost] [$Hridx] [$Hcode] [$HPC] [HKVS Hridx_empty Hn0 Hn1 Hn2]").
+        * iPureIntro; lia.
+        * iPureIntro.
+          intros idx0 Hidx0_bound k0 w0 Hidx0.
+          clear Hidx_empty_found.
+          destruct (decide (idx0 = Z.to_nat n)%Z) as [-> | Hidx']; eauto.
+          { rewrite Hm_kwidx in Hidx0; simplify_map_eq; done. }
+          { eapply Hfkey_notin_nfirst; eauto; lia. }
+        * case_decide as Hnone'.
+          { iFrame. exfalso.
+            replace ( (seq 0 (Z.to_nat (n + 1))) ) with ( (seq 0 (Z.to_nat n)) ++ [Z.to_nat n] ) in Hnone'.
+            2: {
+              replace [Z.to_nat n] with (seq (Z.to_nat n) 1) by done.
+              rewrite -seq_app.
+              replace (Z.to_nat n + 1) with (Z.to_nat (n + 1)) by lia.
+              done.
+            }
+            apply Forall_app in Hnone' as [_ Hnone'].
+            apply (Forall_singleton _ (Z.to_nat n)) in Hnone'; cbn in *.
+            done. }
+          iExists (Z.to_nat n). iSplit; first (iPureIntro; lia).
+          iFrame.
+          replace (Z.of_nat (Z.to_nat n)) with n by lia. iFrame.
+          iPureIntro; exact Hm_kwidx.
+  Qed.
+
   Lemma KVS_search_spec_in `{KVS : kvsLayout}
     (pc_b pc_e pc_a : Addr)
     (cgp_b cgp_e : Addr)
@@ -66,164 +642,25 @@ Section KVS_search.
         )
       ⊢ WP Seq (Instr Executable) {{ v, ⌜v = HaltedV⌝ → na_own cerise_nais ⊤ }})%I.
   Proof.
-    intros instrs ; subst instrs.
-    iIntros (HsubBounds Hbounds_cgp Hcgp_bound Hpkvs_idx
-               Hrscratch Hridx Hridx_empty Hkey)
-      "(HPC & Hcgp & Hrkey & [%widx Hridx] & [%widx_empty Hridx_empty] & Hrscratch
-      & HKVS & Hcode & Hpost)".
-    codefrag_facts "Hcode"; rename H into Hpc_contiguous ; clear H0.
-
-
-    (* mov ridx 0%Z; *)
-    iInstr "Hcode".
-    (* mov ridx_empty (-1)%Z; *)
-    iInstr "Hcode".
-
-    remember 0%Z as n.
-    iAssert (⌜ (0 <= n <= SIZE_MAP)%Z ⌝)%I as "%Hn"; first (iPureIntro ; lia).
-    rewrite{2} (_ : (cgp_b = (cgp_b ^+ (ASM_SIZEOF_KVS_ENTRY * n))%a)); last by solve_addr.
-    assert (forall i, (0 <= i < Z.to_nat n) -> ∀ (k : Z) (w : Word),
-                pkvs !! i = Some (Some (k,w)) -> k ≠ fkey)
-    as Hfkey_notin_nfirst.
-    { rewrite Heqn; intros i Hi; lia. }
-    clear Heqn.
-    generalize ((if decide (ridx_empty = cnull) then (Z.of_nat 0) else (-1)%Z) ); intros nidx_empty.
-
-    iLöb as "IH" forall (n nidx_empty Hn Hfkey_notin_nfirst).
-
-    (* sub rscratch SIZE_MAP ridx; *)
-    iDestruct "Hrscratch" as "[%wrscratch Hrscratch]".
-    iInstr "Hcode".
-    replace 16 with SIZE_MAP by (by rewrite /SIZE_MAP).
-    destruct (decide ((SIZE_MAP - n) = 0)%Z) as [Hneq|Hneq].
-    { (* End of the loop. It means that the key wasn't found in the KVS *)
-      (* We know that it should be a contradiction, because `fkey⤇(KVS) w`
-         witnesses that it exists
-       *)
-      rewrite Hneq.
-      assert ( n = SIZE_MAP ) as -> by lia.
-      iDestruct (kvs_physical_map_indom_idx with "HKVS") as "%Hidx".
-      { by apply elem_of_dom_2 in Hpkvs_idx. }
-      exfalso.
-      eapply Hfkey_notin_nfirst; eauto.
-    }
-    assert (0 ≤ n < SIZE_MAP)%Z as Hn' by lia.
-    (* jnz (".loop_body")%asm rscratch; *)
-    iInstr "Hcode".
-    { by injection. }
-
-    destruct (decide (Z.of_nat idx = n)%Z) as [<- | Hneq'].
-    - iDestruct (kvs_physical_map_open_in with "HKVS") as "(HKVS & Hasm_idx)"; eauto.
-      iDestruct (destruct_physical_kvs_entry_some with "Hasm_idx") as "(Hbk & Hbw & Hfkey)"; first solve_addr.
-
-      (* load rscratch cgp; *)
-      iInstr "Hcode".
-      { split; [done |solve_addr]. }
-      iEval (cbn) in "Hrscratch".
-      (* jnz (".some_index")%asm rscratch; *)
-      iInstr "Hcode".
-
-      (* lea cgp 1; *)
-      iInstr "Hcode".
-      { transitivity (Some ((cgp_b ^+ (ASM_SIZEOF_KVS_ENTRY * idx + 1))%a)); solve_addr. }
-      (* load rscratch cgp; *)
-      iInstr "Hcode".
-      { split; [done |solve_addr]. }
-      iEval (cbn) in "Hrscratch".
-      (* sub rscratch rkey rscratch; *)
-      iInstr "Hcode".
-      replace (fkey - fkey)%Z with 0%Z by (cbn;lia).
-      (* jnz (".not_same_key")%asm rscratch; *)
-      iInstr "Hcode".
-      (* lea cgp (-1)%Z; *)
-      iInstr "Hcode".
-      { transitivity (Some (cgp_b ^+ ASM_SIZEOF_KVS_ENTRY * idx)%a); solve_addr. }
-      (* jmp (".loop_end_found")%asm; *)
-      iInstr "Hcode".
-      iApply "Hpost"; iFrame.
-      iPureIntro; rewrite /withinBounds; solve_addr.
-
-    - iDestruct (kvs_physical_map_open_neq _ _ _ (Z.to_nat n) with "HKVS")
-        as "(%opt_kw' & HKVS & %Hm_idx' & Hkvs_entry & %Hopt_kw')"
-      ; eauto; try lia.
-      iDestruct (destruct_physical_kvs_entry with "Hkvs_entry") as "(Hn0 & Hn1 & Hn2)"; first solve_addr.
-      replace (cgp_b ^+ ASM_SIZEOF_KVS_ENTRY * Z.to_nat n)%a  with (cgp_b ^+ (ASM_SIZEOF_KVS_ENTRY * n))%a by solve_addr+Hn.
-      replace (cgp_b ^+ (ASM_SIZEOF_KVS_ENTRY * Z.to_nat n + 1))%a with (cgp_b ^+ (ASM_SIZEOF_KVS_ENTRY * n + 1))%a by solve_addr+Hn.
-      replace (cgp_b ^+ (ASM_SIZEOF_KVS_ENTRY * Z.to_nat n + 2))%a with (cgp_b ^+ (ASM_SIZEOF_KVS_ENTRY * n + 2))%a by solve_addr+Hn.
-      (* load rscratch cgp; *)
-      iInstr "Hcode".
-      { split; [done | solve_addr]. }
-      iEval (cbn) in "Hrscratch".
-
-      destruct opt_kw' as [ [k' w'] | ].
-      + (* jnz (".some_index")%asm rscratch; *)
-        iInstr "Hcode".
-        (* lea cgp 1; *)
-        iInstr "Hcode".
-        { transitivity (Some ((cgp_b ^+ (ASM_SIZEOF_KVS_ENTRY * n + 1))%a)); last done; solve_addr+Hn Hn' Hcgp_bound. }
-        (* load rscratch cgp; *)
-        iInstr "Hcode".
-        { split; [done | solve_addr]. }
-        (* sub rscratch rkey rscratch; *)
-        iInstr "Hcode".
-        (* jnz (".not_same_key")%asm rscratch; *)
-        iInstr "Hcode".
-        { injection; cbn; intro; apply Hopt_kw'; cbn; lia. }
-        (* lea cgp 2; *)
-        iInstr "Hcode".
-        { transitivity (Some ( (cgp_b ^+ (ASM_SIZEOF_KVS_ENTRY * (n+1)))%a)); last done; solve_addr+Hn Hn' Hcgp_bound. }
-        (* add ridx ridx 1; *)
-        iInstr "Hcode".
-        (* jmp (".loop_start"); *)
-        iInstr "Hcode".
-        { transitivity (Some ( (pc_a ^+ 2)%a)); solve_addr. }
-
-        iDestruct (kvs_physical_map_close with "[$HKVS] [Hn0 Hn1 Hn2]") as "HKVS";eauto.
-        {
-          iApply destruct_physical_kvs_entry; first solve_addr.
-          replace (cgp_b ^+ (ASM_SIZEOF_KVS_ENTRY * n))%a with (cgp_b ^+ ASM_SIZEOF_KVS_ENTRY * Z.to_nat n)%a by solve_addr+Hn.
-          replace (cgp_b ^+ (ASM_SIZEOF_KVS_ENTRY * n + 1))%a  with (cgp_b ^+ (ASM_SIZEOF_KVS_ENTRY * Z.to_nat n + 1))%a by solve_addr+Hn.
-          replace (cgp_b ^+ (ASM_SIZEOF_KVS_ENTRY * n + 2))%a  with (cgp_b ^+ (ASM_SIZEOF_KVS_ENTRY * Z.to_nat n + 2))%a by solve_addr+Hn.
-          iFrame.
-        }
-
-        iApply ("IH" with
-                 "[] [] [$Hcgp] [$Hrkey] [$Hrscratch] [$HKVS] [$Hpost] [$Hridx] [$Hcode] [$HPC] [$Hridx_empty]").
-        * iPureIntro; lia.
-        * iPureIntro.
-          intros idx0 Hidx0_bound k0 w0 Hidx0.
-          destruct (decide (idx0 = Z.to_nat n)%Z) as [-> | Hidx']; eauto.
-          { rewrite Hm_idx' in Hidx0; simplify_map_eq; done. }
-          { eapply Hfkey_notin_nfirst; eauto; lia. }
-      + (* jnz (".some_index")%asm rscratch; *)
-        iInstr "Hcode".
-        (* mov ridx_empty ridx; *)
-        iInstr "Hcode".
-        (* lea cgp ASM_SIZEOF_KVS_ENTRY; *)
-        iInstr "Hcode".
-        { transitivity (Some ((cgp_b ^+ ASM_SIZEOF_KVS_ENTRY * (n + 1))%a)); solve_addr+Hn Hn' Hcgp_bound. }
-        (* add ridx ridx 1; *)
-        iInstr "Hcode".
-        (* jmp (".loop_start"); *)
-        iInstr "Hcode".
-        { transitivity (Some ( (pc_a ^+ 2)%a)); solve_addr. }
-        iDestruct (kvs_physical_map_close with "[$HKVS] [Hn0 Hn1 Hn2]") as "HKVS";eauto.
-        {
-          iApply destruct_physical_kvs_entry; first solve_addr.
-          replace (cgp_b ^+ (ASM_SIZEOF_KVS_ENTRY * n))%a with (cgp_b ^+ ASM_SIZEOF_KVS_ENTRY * Z.to_nat n)%a by solve_addr+Hn.
-          replace (cgp_b ^+ (ASM_SIZEOF_KVS_ENTRY * n + 1))%a  with (cgp_b ^+ (ASM_SIZEOF_KVS_ENTRY * Z.to_nat n + 1))%a by solve_addr+Hn.
-          replace (cgp_b ^+ (ASM_SIZEOF_KVS_ENTRY * n + 2))%a  with (cgp_b ^+ (ASM_SIZEOF_KVS_ENTRY * Z.to_nat n + 2))%a by solve_addr+Hn.
-          iFrame.
-        }
-
-        iApply ("IH" with
-                 "[] [] [$Hcgp] [$Hrkey] [$Hrscratch] [$HKVS] [$Hpost] [$Hridx] [$Hcode] [$HPC] [$Hridx_empty]").
-        * iPureIntro; lia.
-        * iPureIntro.
-          intros idx0 Hidx0_bound k0 w0 Hidx0.
-          destruct (decide (idx0 = Z.to_nat n)%Z) as [-> | Hidx']; eauto.
-          { rewrite Hm_idx' in Hidx0; simplify_map_eq; done. }
-          { eapply Hfkey_notin_nfirst; eauto; lia. }
+    intros instrs HsubBounds Hbounds_cgp Hcgp_bound Hlookup Hrscratch Hridx_ne Hridx_empty_ne Hrkey_ne.
+    iIntros "(HPC & HcgpReg & Hrkey & Hridx & Hridx_empty & HscratchReg & HKVS & Hcode & Hpost)".
+    iDestruct (is_physical_kvs_wf with "HKVS") as %Hwf.
+    iApply (KVS_search_unified_spec pc_b pc_e pc_a cgp_b cgp_e
+      rkey ridx ridx_empty rscratch pkvs fkey
+      HsubBounds Hbounds_cgp Hcgp_bound Hrscratch Hridx_ne Hridx_empty_ne Hrkey_ne
+      with "[$HPC $HcgpReg $Hrkey $Hridx $Hridx_empty $HscratchReg $HKVS $Hcode Hpost]").
+    iNext. iIntros "Houtcome".
+    rewrite /kvs_search_outcome_resources.
+    iDestruct "Houtcome" as "[Hfound | [%Hnotin Hmissing]]".
+    - iDestruct "Hfound" as (idx' w') "(%Hlookup' & Hfound)".
+      destruct (decide (idx = idx')) as [-> | Hidxneq].
+      2: { exfalso.
+           eapply (wf_kvs_neq pkvs idx idx' fkey fkey w w'); eauto. }
+      rewrite Hlookup in Hlookup'; simplify_map_eq.
+      iApply "Hpost".
+      iEval (rewrite /kvs_search_found_resources) in "Hfound". iFrame.
+    - exfalso. apply Hnotin. apply elem_of_kvs_keys.
+      eexists w, idx; exact Hlookup.
   Qed.
 
   Lemma KVS_search_spec_empty_slot `{KVS : kvsLayout}
@@ -296,322 +733,20 @@ Section KVS_search.
         )
       ⊢ WP Seq (Instr Executable) {{ v, ⌜v = HaltedV⌝ → na_own cerise_nais ⊤ }})%I.
   Proof.
-    intros instrs fkey ; subst instrs.
-    iIntros (HsubBounds Hbounds_cgp Hcgp_bound Hs' Hwf_full_key Hrscratch Hridx Hridx_empty Hkey)
-      "(HPC & Hcgp & Hrkey & [%wridx Hridx] & [%wridx_empty Hridx_empty] & Hrscratch
-        & HKVS & Hcode & Hpost)".
-    codefrag_facts "Hcode"; rename H into Hpc_contiguous ; clear H0.
-
-    (* mov ridx 0%Z; *)
-    iInstr "Hcode".
-    (* mov ridx_empty (-1)%Z; *)
-    iInstr "Hcode".
-    destruct (decide (ridx_empty = cnull)) as [|_]; first done.
-    remember (-1)%Z as idx_empty.
-    rewrite {1}Heqidx_empty.
-    rewrite {1}Heqidx_empty.
-    rewrite {1}Heqidx_empty.
-
-    remember 0%Z as n.
-    iAssert (⌜ (0 <= n <= SIZE_MAP)%Z ⌝)%I as "%Hn"; first (iPureIntro ; lia).
-    rewrite{2} (_ : cgp_b = (cgp_b ^+ (ASM_SIZEOF_KVS_ENTRY * n))%a); last by solve_addr.
-    assert (forall i, (0 <= i < Z.to_nat n) -> ∀ (k : Z) (w : Word), pkvs !! i = Some (Some (k,w)) -> k ≠ fkey)
-    as Hfkey_notin_nfirst.
-    { rewrite Heqn; intros i Hi; lia. }
-
-    iAssert (
-       if (decide ((Forall (fun idx => pkvs !! idx ≠ Some None) (seq 0 (Z.to_nat n)))))
-       then (is_physical_kvs cgp_b pkvs ∗
-             ridx_empty ↦ᵣ WInt (-1)
-            )
-       else ( ∃ (idx_empty : nat),
-                ⌜ 0 <= idx_empty < (Z.to_nat n)⌝ ∗
-                is_physical_kvs_open cgp_b pkvs idx_empty ∗
-                (cgp_b ^+ ASM_SIZEOF_KVS_ENTRY * idx_empty)%a ↦ₐ WInt ASM_NONE ∗
-                (cgp_b ^+ (ASM_SIZEOF_KVS_ENTRY * idx_empty + 1))%a ↦ₐ - ∗
-                (cgp_b ^+ (ASM_SIZEOF_KVS_ENTRY * idx_empty + 2))%a ↦ₐ - ∗
-                ridx_empty ↦ᵣ WInt idx_empty ∗
-                ⌜ pkvs !! idx_empty = Some None ⌝
-            )
-      )%I with "[HKVS Hridx_empty]" as "Hloop_inv".
-    {
-      destruct ( decide (Forall (λ idx : nat, pkvs !! idx ≠ Some None) (seq 0 (Z.to_nat n))) ) as [|Hcontra]; rewrite Heqidx_empty; iFrame.
-      exfalso; apply Hcontra.
-      rewrite Heqn /=; apply Forall_nil; done.
-    }
-    clear Heqn Heqidx_empty.
-
-    iLöb as "IH" forall (n Hn Hfkey_notin_nfirst).
-
-    (* sub rscratch SIZE_MAP ridx; *)
-    iDestruct "Hrscratch" as "[%wrscratch Hrscratch]".
-    iInstr "Hcode".
-    replace 16 with SIZE_MAP by (by rewrite /SIZE_MAP).
-    destruct (decide ((SIZE_MAP - n) = 0)%Z) as [Hneq|Hneq].
-    { (* End of the loop. *)
-      rewrite Hneq.
-      assert ( n = SIZE_MAP ) as -> by lia.
-
-      (* jnz (".loop_body")%asm rscratch; *)
-      iInstr "Hcode".
-      (* jmp (".loop_end_not_found")%asm; *)
-      iInstr "Hcode".
-      (* lea cgp (-(ASM_SIZEOF_KVS_ENTRY*SIZE_MAP))%Z; *)
-      iInstr "Hcode".
-      { transitivity (Some cgp_b); rewrite /SIZE_MAP in Hcgp_bound |- *; solve_addr. }
-      (* mov ridx (-1)%Z; *)
-      iInstr "Hcode".
-      rewrite (decide_False (Z.of_nat 0)); last done.
-
-      destruct ( decide ( (Forall (λ idx : nat, pkvs !! idx ≠ Some None) (seq 0 (Z.to_nat SIZE_MAP))) )) as [Hnone|Hnone].
-      - iDestruct "Hloop_inv" as "(HKVS & Hridx_empty)".
-        iApply "Hpost"; iRight; iFrame.
-
-      - iDestruct "Hloop_inv" as
-          "(%idx_empty_found & %Hidx_empty_found & HKVS & Hn0 & Hn1 & Hn2 & Hfkey & Hridx_empty)".
-        iApply "Hpost"; iLeft; iFrame.
-        iPureIntro; split; solve_addr.
-    }
-    assert (0 ≤ n < SIZE_MAP)%Z as Hn' by lia.
-    (* jnz (".loop_body")%asm rscratch; *)
-    iInstr "Hcode".
-    { by injection. }
-
-    destruct ( decide (Forall (λ idx : nat, pkvs !! idx ≠ Some None) (seq 0 (Z.to_nat n))) ) as [Hnone | Hnone].
-    - (* No empty slot have been found yet *)
-      iDestruct "Hloop_inv" as "(HKVS & Hridx_empty)".
-
-      iDestruct (kvs_physical_map_open_notin _ _ (Z.to_nat n) with "HKVS")
-        as "(%opt_kwidx & %Hm_kwidx & HKVS & Hfkey & %Hneq_fkey)" ; eauto; [lia|].
-      iDestruct (destruct_physical_kvs_entry with "Hfkey") as "(Hn0 & Hn1 & Hn2)"; first solve_addr.
-      replace (cgp_b ^+ ASM_SIZEOF_KVS_ENTRY * Z.to_nat n)%a  with (cgp_b ^+ (ASM_SIZEOF_KVS_ENTRY * n))%a by solve_addr+Hn.
-      replace (cgp_b ^+ (ASM_SIZEOF_KVS_ENTRY * Z.to_nat n + 1))%a with (cgp_b ^+ (ASM_SIZEOF_KVS_ENTRY * n + 1))%a by solve_addr+Hn.
-      replace (cgp_b ^+ (ASM_SIZEOF_KVS_ENTRY * Z.to_nat n + 2))%a with (cgp_b ^+ (ASM_SIZEOF_KVS_ENTRY * n + 2))%a by solve_addr+Hn.
-
-      (* load rscratch cgp; *)
-      iInstr "Hcode".
-      { split; [done |solve_addr]. }
-      iEval (cbn) in "Hrscratch".
-
-      destruct opt_kwidx as [ [kidx widx] | ].
-      + (* This is not an empty slot. Because we mkow that fkey ∉ s, the key will not match *)
-        (* jnz (".some_index")%asm rscratch; *)
-        iInstr "Hcode".
-
-        (* lea cgp 1; *)
-        iInstr "Hcode".
-        { transitivity (Some ((cgp_b ^+ (ASM_SIZEOF_KVS_ENTRY * n + 1))%a)); last done; solve_addr+Hn Hn' Hcgp_bound. }
-        (* load rscratch cgp; *)
-        iInstr "Hcode".
-        { split; [done |solve_addr]. }
-        (* sub rscratch rkey rscratch; *)
-        iInstr "Hcode".
-        assert ( WInt (fkey - kidx)%Z ≠ WInt 0 ) as Hfkey_neq.
-        { injection; intro; simplify_eq; apply Hneq_fkey; cbn; lia. }
-        (* jnz (".not_same_key")%asm rscratch; *)
-        iInstr "Hcode".
-
-        (* lea cgp 2; *)
-        iInstr "Hcode".
-        { transitivity (Some ((cgp_b ^+ (ASM_SIZEOF_KVS_ENTRY * n + ASM_SIZEOF_KVS_ENTRY))%a)) ; last done; solve_addr+Hn Hn' Hcgp_bound. }
-        (* add ridx ridx 1; *)
-        iInstr "Hcode".
-        (* jmp (".loop_start"); *)
-        iInstr "Hcode".
-        { transitivity (Some ( (pc_a ^+ 2)%a)); solve_addr. }
-
-        iDestruct (kvs_physical_map_close with "[$HKVS] [Hn0 Hn1 Hn2]") as "HKVS";eauto.
-        {
-          iApply destruct_physical_kvs_entry; first solve_addr.
-          replace (cgp_b ^+ (ASM_SIZEOF_KVS_ENTRY * n))%a with (cgp_b ^+ ASM_SIZEOF_KVS_ENTRY * Z.to_nat n)%a by solve_addr+Hn.
-          replace (cgp_b ^+ (ASM_SIZEOF_KVS_ENTRY * n + 1))%a  with (cgp_b ^+ (ASM_SIZEOF_KVS_ENTRY * Z.to_nat n + 1))%a by solve_addr+Hn.
-          replace (cgp_b ^+ (ASM_SIZEOF_KVS_ENTRY * n + 2))%a  with (cgp_b ^+ (ASM_SIZEOF_KVS_ENTRY * Z.to_nat n + 2))%a by solve_addr+Hn.
-          iFrame.
-        }
-        replace (cgp_b ^+ (ASM_SIZEOF_KVS_ENTRY * n + ASM_SIZEOF_KVS_ENTRY))%a with (cgp_b ^+ (ASM_SIZEOF_KVS_ENTRY * (n + 1)))%a by solve_addr+ Hn Hn' Hcgp_bound.
-
-        iApply ("IH" with "[] [] [$Hcgp] [$Hrkey] [$Hrscratch]
-         [$Hpost] [$Hridx] [$Hcode] [$HPC] [HKVS Hridx_empty]").
-        * iPureIntro; lia.
-        * iPureIntro.
-          intros idx0 Hidx0_bound k0 w0 Hidx0.
-          destruct (decide (idx0 = Z.to_nat n)%Z) as [-> | Hidx']; eauto.
-          { rewrite Hm_kwidx in Hidx0; simplify_map_eq; done. }
-          { eapply Hfkey_notin_nfirst; eauto; lia. }
-        * case_decide as Hnone'; iFrame.
-          exfalso.
-          apply Hnone'.
-          replace ( (seq 0 (Z.to_nat (n + 1))) ) with ( (seq 0 (Z.to_nat n)) ++ [Z.to_nat n] ).
-          2: {
-            replace [Z.to_nat n] with (seq (Z.to_nat n) 1) by done.
-            rewrite -seq_app.
-            replace (Z.to_nat n + 1) with (Z.to_nat (n + 1)) by lia.
-            done.
-          }
-          apply Forall_app; split; auto.
-          apply Forall_singleton.
-          rewrite Hm_kwidx; done.
-      + (* This is an empty slot. We will update ridx_empty and keep KVS open *)
-
-        (* jnz (".some_index")%asm rscratch; *)
-        iInstr "Hcode".
-        (* mov ridx_empty ridx; *)
-        iInstr "Hcode".
-        (* lea cgp ASM_SIZEOF_KVS_ENTRY; *)
-        iInstr "Hcode".
-        { transitivity (Some ((cgp_b ^+ (ASM_SIZEOF_KVS_ENTRY * (n + 1)))%a)); solve_addr+Hn Hn' Hcgp_bound. }
-        (* add ridx ridx 1; *)
-        iInstr "Hcode".
-        (* jmp (".loop_start"); *)
-        iInstr "Hcode".
-        { transitivity (Some ( (pc_a ^+ 2)%a)); solve_addr. }
-
-        rewrite {5}(_ : n = (Z.of_nat (Z.to_nat n))); last lia.
-        replace (cgp_b ^+ (ASM_SIZEOF_KVS_ENTRY * n))%a with (cgp_b ^+ ASM_SIZEOF_KVS_ENTRY * Z.to_nat n)%a by solve_addr+Hn.
-        replace (cgp_b ^+ (ASM_SIZEOF_KVS_ENTRY * n + 1))%a  with (cgp_b ^+ (ASM_SIZEOF_KVS_ENTRY * Z.to_nat n + 1))%a by solve_addr+Hn.
-        replace (cgp_b ^+ (ASM_SIZEOF_KVS_ENTRY * n + 2))%a  with (cgp_b ^+ (ASM_SIZEOF_KVS_ENTRY * Z.to_nat n + 2))%a by solve_addr+Hn.
-        iApply ("IH" with "[] [] [$Hcgp] [$Hrkey] [$Hrscratch]
-         [$Hpost] [$Hridx] [$Hcode] [$HPC] [HKVS Hridx_empty Hn0 Hn1 Hn2]").
-        * iPureIntro; lia.
-        * iPureIntro.
-          intros idx0 Hidx0_bound k0 w0 Hidx0.
-          destruct (decide (idx0 = Z.to_nat n)%Z) as [-> | Hidx']; eauto.
-          { rewrite Hm_kwidx in Hidx0; simplify_map_eq; done. }
-          { eapply Hfkey_notin_nfirst; eauto; lia. }
-        * case_decide as Hnone'; iFrame; last (iPureIntro; split; auto; lia).
-          exfalso.
-          replace ( (seq 0 (Z.to_nat (n + 1))) ) with ( (seq 0 (Z.to_nat n)) ++ [Z.to_nat n] ) in Hnone'.
-          2: {
-            replace [Z.to_nat n] with (seq (Z.to_nat n) 1) by done.
-            rewrite -seq_app.
-            replace (Z.to_nat n + 1) with (Z.to_nat (n + 1)) by lia.
-            done.
-          }
-          apply Forall_app in Hnone' as [_ Hnone'].
-          apply (Forall_singleton _ (Z.to_nat n)) in Hnone'; cbn in *.
-          done.
-
-    - (* An empty slot have already been found *)
-      iDestruct "Hloop_inv" as
-        "(%idx_empty_found & %Hidx_empty_found & HKVS & Hn0 & Hn1 & Hn2 & Hridx_empty
-          & %Hpkvs_idx_empty)".
-
-      iDestruct (kvs_physical_map_close _ _ _ None with "[$HKVS] [Hn0 Hn1 Hn2]") as "HKVS";eauto.
-      { iApply destruct_physical_kvs_entry; first solve_addr; iFrame. }
-
-
-      iDestruct (kvs_physical_map_open_notin _ _ (Z.to_nat n) with "HKVS")
-        as "(%opt_kwidx & %Hm_kwidx & HKVS & Hfkey & %Hneq_fkey)" ; eauto; [lia|].
-      iDestruct (destruct_physical_kvs_entry with "Hfkey") as "(Hn0 & Hn1 & Hn2)"; first solve_addr.
-      replace (cgp_b ^+ ASM_SIZEOF_KVS_ENTRY * Z.to_nat n)%a  with (cgp_b ^+ (ASM_SIZEOF_KVS_ENTRY * n))%a by solve_addr+Hn.
-      replace (cgp_b ^+ (ASM_SIZEOF_KVS_ENTRY * Z.to_nat n + 1))%a with (cgp_b ^+ (ASM_SIZEOF_KVS_ENTRY * n + 1))%a by solve_addr+Hn.
-      replace (cgp_b ^+ (ASM_SIZEOF_KVS_ENTRY * Z.to_nat n + 2))%a with (cgp_b ^+ (ASM_SIZEOF_KVS_ENTRY * n + 2))%a by solve_addr+Hn.
-
-      (* load rscratch cgp; *)
-      iInstr "Hcode".
-      { split; [done |solve_addr]. }
-      iEval (cbn) in "Hrscratch".
-
-
-      destruct opt_kwidx as [ [kidx widx] | ].
-      + (* This is not an empty slot. Because we mkow that fkey ∉ s, the key will not match *)
-        (* jnz (".some_index")%asm rscratch; *)
-        iInstr "Hcode".
-
-        (* lea cgp 1; *)
-        iInstr "Hcode".
-        { transitivity (Some ((cgp_b ^+ (ASM_SIZEOF_KVS_ENTRY * n + 1))%a)); last done; solve_addr+Hn Hn' Hcgp_bound. }
-        (* load rscratch cgp; *)
-        iInstr "Hcode".
-        { split; [done |solve_addr]. }
-        (* sub rscratch rkey rscratch; *)
-        iInstr "Hcode".
-        assert ( WInt (fkey - kidx)%Z ≠ WInt 0 ) as Hfkey_neq.
-        { injection; intro; simplify_eq; apply Hneq_fkey; cbn; lia. }
-        (* jnz (".not_same_key")%asm rscratch; *)
-        iInstr "Hcode".
-
-        (* lea cgp 2; *)
-        iInstr "Hcode".
-        { transitivity (Some ((cgp_b ^+ (ASM_SIZEOF_KVS_ENTRY * n + ASM_SIZEOF_KVS_ENTRY))%a)) ; last done; solve_addr+Hn Hn' Hcgp_bound. }
-        (* add ridx ridx 1; *)
-        iInstr "Hcode".
-        (* jmp (".loop_start"); *)
-        iInstr "Hcode".
-        { transitivity (Some ( (pc_a ^+ 2)%a)); solve_addr. }
-
-        iDestruct (kvs_physical_map_close with "[$HKVS] [Hn0 Hn1 Hn2]") as "HKVS";eauto.
-        {
-          iApply destruct_physical_kvs_entry; first solve_addr.
-          replace (cgp_b ^+ (ASM_SIZEOF_KVS_ENTRY * n))%a with (cgp_b ^+ ASM_SIZEOF_KVS_ENTRY * Z.to_nat n)%a by solve_addr+Hn.
-          replace (cgp_b ^+ (ASM_SIZEOF_KVS_ENTRY * n + 1))%a  with (cgp_b ^+ (ASM_SIZEOF_KVS_ENTRY * Z.to_nat n + 1))%a by solve_addr+Hn.
-          replace (cgp_b ^+ (ASM_SIZEOF_KVS_ENTRY * n + 2))%a  with (cgp_b ^+ (ASM_SIZEOF_KVS_ENTRY * Z.to_nat n + 2))%a by solve_addr+Hn.
-          iFrame.
-        }
-        replace (cgp_b ^+ (ASM_SIZEOF_KVS_ENTRY * n + ASM_SIZEOF_KVS_ENTRY))%a with (cgp_b ^+ (ASM_SIZEOF_KVS_ENTRY * (n + 1)))%a by solve_addr + Hn Hn' Hcgp_bound.
-
-        iDestruct (kvs_physical_map_open_notin _ _ idx_empty_found with "HKVS")
-          as "(%opt_kwidx_empty & %Hm_kwidx_empty & HKVS & Hfkey & %Hneq_fkey_empty)" ; eauto; [lia|].
-        rewrite Hpkvs_idx_empty in Hm_kwidx_empty; simplify_eq.
-        iDestruct (destruct_physical_kvs_entry with "Hfkey") as "(Hn0 & Hn1 & Hn2)"; first solve_addr.
-
-        iApply ("IH" with "[] [] [$Hcgp] [$Hrkey] [$Hrscratch]
-         [$Hpost] [$Hridx] [$Hcode] [$HPC] [HKVS Hn0 Hn1 Hn2 Hridx_empty]").
-        * iPureIntro; lia.
-        * iPureIntro.
-          intros idx0 Hidx0_bound k0 w0 Hidx0.
-          clear Hidx_empty_found.
-          destruct (decide (idx0 = Z.to_nat n)%Z) as [-> | Hidx']; eauto.
-          { rewrite Hm_kwidx in Hidx0; simplify_map_eq; done. }
-          { eapply Hfkey_notin_nfirst; eauto; lia. }
-        * case_decide as Hnone'; iFrame; last (iPureIntro; split; auto; lia).
-          exfalso.
-          rewrite Forall_forall in Hnone'.
-          specialize (Hnone' idx_empty_found).
-          apply Hnone'; auto.
-          apply elem_of_seq; lia.
-
-
-      + (* This is an empty slot. We will update ridx_empty and keep KVS open *)
-
-        (* jnz (".some_index")%asm rscratch; *)
-        iInstr "Hcode".
-        (* mov ridx_empty ridx; *)
-        iInstr "Hcode".
-        (* lea cgp ASM_SIZEOF_KVS_ENTRY; *)
-        iInstr "Hcode".
-        { transitivity (Some ((cgp_b ^+ (ASM_SIZEOF_KVS_ENTRY * (n + 1)))%a)); solve_addr+Hn Hn' Hcgp_bound. }
-        (* add ridx ridx 1; *)
-        iInstr "Hcode".
-        (* jmp (".loop_start"); *)
-        iInstr "Hcode".
-        { transitivity (Some ( (pc_a ^+ 2)%a)); solve_addr. }
-
-        rewrite {5}(_ : n = (Z.of_nat (Z.to_nat n))); last lia.
-        replace (cgp_b ^+ (ASM_SIZEOF_KVS_ENTRY * n))%a with (cgp_b ^+ ASM_SIZEOF_KVS_ENTRY * Z.to_nat n)%a by solve_addr+Hn.
-        replace (cgp_b ^+ (ASM_SIZEOF_KVS_ENTRY * n + 1))%a  with (cgp_b ^+ (ASM_SIZEOF_KVS_ENTRY * Z.to_nat n + 1))%a by solve_addr+Hn.
-        replace (cgp_b ^+ (ASM_SIZEOF_KVS_ENTRY * n + 2))%a  with (cgp_b ^+ (ASM_SIZEOF_KVS_ENTRY * Z.to_nat n + 2))%a by solve_addr+Hn.
-        iApply ("IH" with "[] [] [$Hcgp] [$Hrkey] [$Hrscratch]
-         [$Hpost] [$Hridx] [$Hcode] [$HPC] [HKVS Hridx_empty Hn0 Hn1 Hn2]").
-        * iPureIntro; lia.
-        * iPureIntro.
-          intros idx0 Hidx0_bound k0 w0 Hidx0.
-          clear Hidx_empty_found.
-          destruct (decide (idx0 = Z.to_nat n)%Z) as [-> | Hidx']; eauto.
-          { rewrite Hm_kwidx in Hidx0; simplify_map_eq; done. }
-          { eapply Hfkey_notin_nfirst; eauto; lia. }
-        * case_decide as Hnone'; iFrame; last (iPureIntro; split; auto; lia).
-          exfalso.
-          replace ( (seq 0 (Z.to_nat (n + 1))) ) with ( (seq 0 (Z.to_nat n)) ++ [Z.to_nat n] ) in Hnone'.
-          2: {
-            replace [Z.to_nat n] with (seq (Z.to_nat n) 1) by done.
-            rewrite -seq_app.
-            replace (Z.to_nat n + 1) with (Z.to_nat (n + 1)) by lia.
-            done.
-          }
-          apply Forall_app in Hnone' as [_ Hnone'].
-          apply (Forall_singleton _ (Z.to_nat n)) in Hnone'; cbn in *.
-          done.
+    intros instrs fkey HsubBounds Hbounds_cgp Hcgp_bound Hnotin Huint16
+      Hrscratch Hridx_ne Hridx_empty_ne Hrkey_ne.
+    iIntros "(HPC & HcgpReg & Hrkey & Hridx & Hridx_empty & HscratchReg & HKVS & Hcode & Hpost)".
+    iApply (KVS_search_unified_spec pc_b pc_e pc_a cgp_b cgp_e
+      rkey ridx ridx_empty rscratch pkvs fkey
+      HsubBounds Hbounds_cgp Hcgp_bound Hrscratch Hridx_ne Hridx_empty_ne Hrkey_ne
+      with "[$HPC $HcgpReg $Hrkey $Hridx $Hridx_empty $HscratchReg $HKVS $Hcode Hpost]").
+    iNext. iIntros "Houtcome".
+    rewrite /kvs_search_outcome_resources.
+    iDestruct "Houtcome" as "[Hfound | [_ Hmissing]]".
+    - iDestruct "Hfound" as (idx' w') "(%Hlookup & _)".
+      exfalso. apply Hnotin. apply elem_of_kvs_keys.
+      eexists w', idx'; exact Hlookup.
+    - iApply "Hpost".
+      iEval (rewrite /kvs_search_missing_resources) in "Hmissing". iFrame.
   Qed.
-
 End KVS_search.
